code/ecdsa/Hacl.Impl.EC.Exponent.fst
@@ -1,0 +1,58 @@
+module Hacl.Impl.EC.Exponent
+
+open FStar.HyperStack.All
+open FStar.HyperStack
+module ST = FStar.HyperStack.ST
+
+open Hacl.Impl.P256.Math 
+
+open Lib.IntTypes
+open Lib.Buffer
+
+open FStar.Math.Lemmas
+open FStar.Mul
+
+open Hacl.Spec.P256.Definition
+open Hacl.Lemmas.P256
+open Spec.P256
+open Spec.ECDSA.Lemmas
+
+open Hacl.Impl.EC.LowLevel
+
+open Lib.Loops
+open Hacl.Spec.P.MontgomeryMultiplication
+
+open Hacl.Impl.EC.MontgomeryMultiplication
+open Hacl.Impl.P256.MontgomeryMultiplication.Exponent
+open Hacl.Impl.MM.Exponent
+
+
+
+let exponent #c a result tempBuffer = 
+  match c with 
+  |P384 ->
+    recall_contents (prime_inverse_buffer #c) (prime_inverse_seq #c);
+    montgomery_ladder_power #c a prime_inverse_buffer result
+  |P256 -> 
+    exponent_p256 a result tempBuffer
+
+
+inline_for_extraction
+let sqPower_buffer_p256 : x: glbuffer uint8 (getScalarLen P256) {witnessed x sqPower_seq /\ recallable x} = 
+  createL_global sqPower_list_p256
+
+
+inline_for_extraction
+let sqPower_buffer_p384 : x: glbuffer uint8 (getScalarLen P384) {witnessed x sqPower_seq /\ recallable x} = 
+  createL_global sqPower_list_p384
+
+inline_for_extraction
+let sqPower_buffer (#c: curve): (x: glbuffer uint8 (getScalarLen c)) = 
+  match c with
+  |P256 -> sqPower_buffer_p256 
+  |P384 -> sqPower_buffer_p384 
+
+
+let square_root #c a result = 
+  recall_contents (sqPower_buffer #c) (sqPower_seq #c);
+  montgomery_ladder_power a sqPower_buffer result
