code/ecdsa/Hacl.Impl.EC.Exponent.fsti
@@ -1,0 +1,48 @@
+
+module Hacl.Impl.EC.Exponent
+
+open FStar.HyperStack.All
+open FStar.HyperStack
+module ST = FStar.HyperStack.ST
+
+open Hacl.Impl.P256.Math 
+
+open Lib.IntTypes
+open Lib.Buffer
+
+open FStar.Math.Lemmas
+open FStar.Mul
+
+open Hacl.Spec.P256.Definition
+open Hacl.Lemmas.P256
+open Spec.P256
+open Spec.ECDSA.Lemmas
+
+open Hacl.Impl.EC.LowLevel
+
+open Lib.Loops
+open Hacl.Spec.P.MontgomeryMultiplication
+
+open Hacl.Impl.P256.MontgomeryMultiplication.Exponent
+open Hacl.Impl.P256.MontgomeryMultiplication
+open Hacl.Impl.P256.MM.Exponent
+
+open FStar.Mul
+
+
+val exponent: #c: curve -> a: felem c -> result: felem c -> tempBuffer: lbuffer uint64 (getCoordinateLenU64 c *. 8ul) 
+  -> Stack unit
+    (requires fun h -> 
+      live h a /\ live h result /\ as_nat c h a < getPrime c)
+    (ensures fun h0 _ h1 -> 
+      let k = fromDomain_ #c (as_nat c h0 a) in 
+      modifies (loc a |+| loc result) h0 h1 /\
+      as_nat c h1 result = toDomain_ #c (pow k (getPrime c - 2) % getPrime c))
+
+val square_root: #c: curve -> a: felem c -> result: felem c -> Stack unit 
+  (requires fun h -> live h a /\ live h result /\ as_nat c h a < getPrime c)
+  (ensures fun h0 _ h1 -> modifies (loc a |+| loc result) h0 h1 /\
+    as_nat c h1 result < getPrime c /\
+    fromDomain_ #c (as_nat c h1 result) = sq_root_spec #c (fromDomain_ #c (as_nat c h0 a)) /\
+    fromDomain_ #c (as_nat c h1 result) = pow (fromDomain_ #c (as_nat c h0 a)) ((getPrime c + 1) / 4) % getPrime c
+  )
