code/ecdsa/Hacl.Impl.EC.MontgomeryMultiplication.fst
@@ -1,0 +1,54 @@
+module Hacl.Impl.EC.MontgomeryMultiplication
+
+open FStar.HyperStack.All
+open FStar.HyperStack
+module ST = FStar.HyperStack.ST
+
+open Hacl.Impl.P256.Math 
+
+open Lib.IntTypes
+open Lib.Buffer
+
+open FStar.Math.Lemmas
+open FStar.Mul
+
+open Hacl.Spec.P256.Definition
+open Hacl.Lemmas.P256
+open Spec.P256
+open Spec.ECDSA.Lemmas
+
+open Hacl.Impl.EC.LowLevel
+
+open Lib.Loops
+open Hacl.Spec.P.MontgomeryMultiplication
+
+(* open Hacl.Impl.P256.MontgomeryMultiplication.Exponent *)
+open Hacl.Impl.P256.MontgomeryMultiplication
+(* open Hacl.Impl.P256.MM.Exponent *)
+
+
+let montgomery_multiplication_buffer_by_one #c a result = 
+  match c with 
+  |P256 -> 
+    assume ((getPrime c + 1) % pow2 64 == 0);
+    montgomery_multiplication_buffer_by_one_w_ko a result
+  |P384 -> montgomery_multiplication_buffer_by_one_ko a result
+
+
+
+let montgomery_multiplication_buffer #c a b result = 
+  match c with 
+  |P256 ->
+    assume ((getPrime c + 1) % pow2 64 == 0);
+    montgomery_multiplication_buffer_w_k0 a b result
+  |P384 -> montgomery_multiplication_buffer_k0 a b result
+
+
+
+let montgomery_square_buffer #c a result = 
+  match c with 
+  |P256 ->
+     assume ((getPrime c + 1) % pow2 64 == 0);
+     montgomery_square_buffer_w_k0 a result
+  |P384 -> montgomery_square_buffer_k0 a result
+
