code/ecdsa/Hacl.Impl.EC.PointDouble.fst
@@ -1,0 +1,45 @@
+module Hacl.Impl.EC.PointDouble
+
+open FStar.HyperStack.All
+open FStar.HyperStack
+module ST = FStar.HyperStack.ST
+
+open Lib.IntTypes
+open Hacl.Impl.P256.Arithmetics
+
+open Lib.Buffer
+
+open Hacl.Lemmas.P256
+open Hacl.Spec.P256.Definition
+(* open Hacl.Impl.SolinasReduction *)
+open Hacl.Spec.P.MontgomeryMultiplication
+open Hacl.Impl.EC.LowLevel
+open Hacl.Impl.P256.MontgomeryMultiplication
+open Spec.P256
+open Hacl.Impl.P256.Math 
+
+open Hacl.Impl.P.PointDouble
+
+
+val point_double: #c: curve -> p: point c -> result: point c 
+  -> tempBuffer: lbuffer uint64  (getCoordinateLenU64 c *! 17ul) 
+  -> Stack unit
+    (requires fun h -> live h p /\ live h tempBuffer /\ live h result /\
+      disjoint p tempBuffer /\ disjoint result tempBuffer /\
+      eq_or_disjoint p result /\ point_eval c h p)
+  (ensures fun h0 _ h1 -> modifies (loc tempBuffer |+| loc result) h0 h1 /\  
+    (
+      point_eval c h1 result /\ (
+      
+      let x, y, z = point_x_as_nat c h0 p, point_y_as_nat c h0 p, point_z_as_nat c h0 p in 
+      let x3, y3, z3 = point_x_as_nat c h1 result, point_y_as_nat c h1 result, point_z_as_nat c h1 result in       
+      let xD, yD, zD = fromDomain_ #c x, fromDomain_ #c y, fromDomain_ #c z in 
+      let x3D, y3D, z3D = fromDomain_ #c x3, fromDomain_ #c y3, fromDomain_ #c z3 in
+      let xN, yN, zN = _point_double #c (xD, yD, zD) in 
+      x3D == xN /\ y3D == yN /\ z3D == zN )))
+
+
+let point_double #c p result tempBuffer = 
+	match c with 
+	|P256 -> Hacl.Impl.P.PointDouble.point_double p result tempBuffer
+	|P384 -> Hacl.Impl.P.PointDouble.point_double p result tempBuffer
