code/ecdsa/Hacl.Impl.P256.Arithmetics.fst
@@ -11,7 +11,7 @@ open Hacl.Lemmas.P256
 open Hacl.Spec.P256.Definition
 
 open Hacl.Impl.EC.LowLevel
-open Hacl.Impl.P256.MontgomeryMultiplication
+open Hacl.Impl.EC.MontgomeryMultiplication
 open Spec.P256
 
 open Hacl.Spec.P.MontgomeryMultiplication
